add normalization of stlc

theories/stlc_cbv.v
@@ -2,7 +2,7 @@ From Coq.Unicode Require Import Utf8.
 From Coq.Lists Require Import List.
 From Autosubst Require Import Autosubst.
 From Coq.Relations Require Import Relations.
-From ShortLogrels Require Import prelude.
+From ShortLogrels Require Import prelude language.
 
 Inductive expr :=
 | Var (v : var)
@@ -188,75 +188,3 @@ Ltac solve_det_head_step :=
   solve [eapply det_head_step_fst; assumption|
           eapply det_head_step_snd; assumption|
           eapply det_head_step_app; eassumption].
-
-Fixpoint val_rel (τ : type) (v : expr) : Prop :=
-  match τ with
-  | TUnit => v = TT
-  | TProd τ1 τ2 => ∃ v1 v2, v = Pair v1 v2 ∧ val_rel τ1 v1 ∧ val_rel τ2 v2
-  | TFun τ1 τ2 => is_val v ∧ ∀ w, val_rel τ1 w → Safe (val_rel τ2) (App v w)
-  end.
-
-Lemma val_rel_is_val τ v : val_rel τ v → is_val v.
-Proof.
-  revert v; induction τ; intros v; simpl in *; subst.
-  - intros ?; subst; constructor.
-  - firstorder; subst; constructor; auto.
-  - intuition.
-Qed.
-
-Definition expr_rel (τ : type) (e : expr) := Safe (val_rel τ) e.
-
-Theorem Fundamental Γ e τ :
-  typed Γ e τ → ∀ env, env_rel val_rel Γ env → expr_rel τ e.[env_subst env].
-Proof.
-  intros Htp.
-  induction Htp; intros env Henv; simpl.
-  - simpl.
-    assert (val_rel tp (env_subst env v)).
-    { eapply env_rel_lookup1 in Henv as [? [? ?]]; [|eauto; fail].
-      erewrite env_subst_lookup; eauto. }
-    apply Safe_val; [eapply val_rel_is_val; eauto|assumption].
-  - apply Safe_val; [constructor|simpl; trivial].
-  - eapply (Safe_bind _ _ _ (λ e, Pair e _));
-      [repeat econstructor; fail|apply IHHtp1; trivial; fail|].
-    intros v1 Hv11 Hv12.
-    eapply (Safe_bind _ _ _ (λ e, Pair _ e)); [|apply IHHtp2; trivial; fail|].
-    { repeat econstructor; trivial. }
-    intros v2 Hv21 Hv22.
-    apply Safe_val; [constructor; trivial; fail|eexists _, _; eauto].
-  - eapply (Safe_bind _ _ _ (λ e, Fst e));
-      [repeat econstructor; fail|apply IHHtp; trivial; fail|].
-    intros v Hv1 (v1 & v2 & -> & Hv1r & Hv2r).
-    inversion Hv1; subst.
-    eapply Safe_head_step_back; [solve_det_head_step|].
-    apply Safe_val; assumption.
-  - eapply (Safe_bind _ _ _ (λ e, Snd e));
-      [repeat econstructor; fail|apply IHHtp; trivial; fail|].
-    intros v Hv1 (v1 & v2 & -> & Hv1r & Hv2r).
-    inversion Hv1; subst.
-    eapply Safe_head_step_back; [solve_det_head_step|].
-    apply Safe_val; assumption.
-  - apply Safe_val; [constructor; fail|].
-    split; [constructor; fail|].
-    intros w Hw.
-    assert (is_val w) by (eapply val_rel_is_val; eauto).
-    eapply Safe_head_step_back; [solve_det_head_step|].
-    asimpl.
-    apply (IHHtp (_ :: _)).
-    apply env_rel_cons; assumption.
-  - eapply (Safe_bind _ _ _ (λ e, App e _));
-      [repeat econstructor; fail|apply IHHtp1; trivial; fail|].
-    intros v1 Hv11 Hv12.
-    eapply (Safe_bind _ _ _ (λ e, App _ e)); [|apply IHHtp2; trivial; fail|].
-    { repeat econstructor; trivial. }
-    intros v2 Hv21 Hv22.
-    apply Hv12; trivial.
-Qed.
-
-Corollary type_safety e τ : typed nil e τ → Safe (λ _, True) e.
-Proof.
-  intros Htp.
-  eapply Safe_mono; [tauto|].
-  replace e with e.[env_subst nil] by (asimpl; reflexivity).
-  eapply (Fundamental nil); [eassumption|apply env_rel_nil].
-Qed.
