theories/language.v
@@ -1,0 +1,270 @@
+From Coq.Unicode Require Import Utf8.
+From Coq.Lists Require Import List.
+From Coq.Relations Require Import Relations.
+
+Class valid_language {expr : Type}
+    (is_val : expr → Prop)
+    (is_ectx : (expr → expr) → Prop)
+    (head_step : expr → expr → Prop) : Type :=
+ValidLang {
+  is_val_no_head_step : ∀ v, is_val v → ∀ e', ¬ head_step v e';
+  is_val_under_ectx : ∀ e K , is_ectx K → is_val (K e) → is_val e;
+  is_ectx_id : is_ectx (λ e, e);
+  is_val_dec : ∀ e, is_val e ∨ ¬ is_val e;
+  ectx_head_step : ∀ K e e', is_ectx K → head_step (K e) e' → (∀ f, K f = f) ∨ is_val e;
+  ectx_inj : ∀ K e e', is_ectx K → K e = K e' → e = e';
+  ectx_compose : ∀ K K', is_ectx K → is_ectx K' → is_ectx (λ e, K (K' e));
+  ectxs_nesting : ∀ K e K' e',
+      is_ectx K →
+      is_ectx K' →
+      K e = K' e' →
+      ¬ is_val e →
+      ¬ is_val e' →
+      (∃ K'', is_ectx K'' ∧ ∀ f, K f = K' (K'' f)) ∨ (∃ K'', is_ectx K'' ∧ ∀ f, K' f = K (K'' f))
+}.
+
+Inductive step {expr is_val is_ectx head_step} `{@valid_language expr is_val is_ectx head_step} :
+  expr → expr → Prop :=
+| Step K e1 e2 : is_ectx K → head_step e1 e2 → step (K e1) (K e2).
+
+Definition steps {expr is_val is_ectx head_step} `{@valid_language expr is_val is_ectx head_step} :=
+  clos_refl_trans _ step.
+
+Definition det_head_step
+  {expr is_val is_ectx head_step} `{@valid_language expr is_val is_ectx head_step} e e' :=
+  head_step e e' ∧ ∀ e'', head_step e e'' → e'' = e'.
+
+Definition det_step
+  {expr is_val is_ectx head_step} `{@valid_language expr is_val is_ectx head_step} e e' :=
+  step e e' ∧ ∀ e'', step e e'' → e'' = e'.
+
+Section language.
+  Context {expr is_val is_ectx head_step} `{@valid_language expr is_val is_ectx head_step}.
+
+  Lemma steps_ind (P : expr → expr → Prop) :
+    (∀ e, P e e) →
+    (∀ e e' e'', step e e' → steps e' e'' → P e' e'' → P e e'') →
+    ∀ e e', steps e e' → P e e'.
+  Proof.
+    intros Hrfl Hstp e e' Hsteps.
+    apply clos_rt_rt1n_iff in Hsteps.
+    induction Hsteps; [apply Hrfl|].
+    eapply Hstp; [eassumption|apply clos_rt_rt1n_iff; assumption|assumption].
+  Qed.
+
+  Lemma steps_refl e : steps e e.
+  Proof. constructor; fail. Qed.
+
+  Lemma step_steps e e' : step e e' → steps e e'.
+  Proof. constructor; assumption. Qed.
+
+  Lemma steps_trans e e' e'' : steps e e' → steps e' e'' → steps e e''.
+  Proof. econstructor; eauto; fail. Qed.
+
+  Lemma val_no_step e : is_val e → ∀ e', ¬ step e e'.
+  Proof.
+    intros He e' Hstp.
+    inversion Hstp as [K e1 e2 HK Hhs]; subst; clear Hstp.
+    apply is_val_under_ectx in He; [|assumption].
+    eapply is_val_no_head_step; eauto.
+  Qed.
+
+  Lemma val_steps_eq e e' : is_val e → steps e e' → e = e'.
+  Proof.
+    induction 2 as [| |???? IH1 ? IH2]; subst; [|trivial; fail|].
+    - exfalso; eapply val_no_step; eauto.
+    - assert (x = y) by (apply IH1; trivial); subst.
+      apply IH2; trivial.
+  Qed.
+
+  Lemma head_step_step e e' : head_step e e' → step e e'.
+  Proof. intros; eapply (Step (λ e, e)); [apply is_ectx_id|assumption]. Qed.
+
+  Lemma ectx_step e e' K : is_ectx K → step e e' → step (K e) (K e').
+  Proof.
+    intros ?; inversion 1 as [K' e1 e2]; subst.
+    eapply (Step (λ e, K (K' e))); [apply ectx_compose; assumption|assumption].
+  Qed.
+
+  Lemma ectx_steps e e' K : is_ectx K → steps e e' → steps (K e) (K e').
+  Proof.
+    intros HK Hstep.
+    pattern e; pattern e'.
+    match goal with
+    | |- (λ e2, (λ e1, ?P) _) _ => simpl; apply (steps_ind (λ e1 e2, P))
+    end; [| |assumption]; clear e e' Hstep.
+    - intros ?; apply steps_refl.
+    - intros e e' e'' Hstep Hsteps HKsteps.
+      eapply steps_trans; [apply step_steps, ectx_step|]; eassumption.
+  Qed.
+
+  Lemma steps_eq_or_step_iff e e' : steps e e' ↔ e = e' ∨ ∃ e'', step e e'' ∧ steps e'' e'.
+  Proof.
+    split.
+    - intros Hsteps; apply clos_rt_rt1n_iff in Hsteps.
+      inversion Hsteps as [|??? Hsteps']; [eauto; fail|].
+      apply clos_rt_rt1n_iff in Hsteps'; eauto.
+    - intros [->|[? [? ?]]]; apply clos_rt_rt1n_iff;
+        [constructor; fail|econstructor; [|apply clos_rt_rt1n_iff]]; eauto.
+  Qed.
+
+  Lemma step_under_ectx K e e' :
+    is_ectx K → step (K e) e' →
+    (is_val e) ∨ (∃ e'', step e e'' ∧ e' = K e'').
+  Proof.
+    intros HK Hstp.
+    destruct (is_val_dec e) as [Hiv|Hniv].
+    - auto.
+    - right.
+      inversion Hstp as [K' e1 e2 HK' Hhs HKe1e]; subst.
+      destruct (ectxs_nesting _ _ _ _ HK' HK HKe1e) as [[K'' [HK''1 HK''2]]|[K'' [HK''1 HK''2]]];
+      [intros ?; contradict Hhs; apply is_val_no_head_step; assumption|assumption| |].
+      + rewrite HK''2 in HKe1e.
+        apply ectx_inj in HKe1e; [|assumption].
+        subst.
+        exists (K'' e2); rewrite HK''2; split; [|reflexivity].
+        constructor; trivial.
+      + rewrite HK''2 in HKe1e.
+        apply ectx_inj in HKe1e; [|assumption].
+        subst.
+        pose proof Hhs as Hhs'.
+        apply ectx_head_step in Hhs as [Hhs|Hhs]; [|tauto|assumption].
+        rewrite Hhs in Hhs'.
+        exists e2; split; [apply head_step_step; assumption|].
+        rewrite HK''2, Hhs; trivial.
+  Qed.
+
+  Definition Safe (P : expr → Prop) (e : expr) :=
+    ∀ e', steps e e' → (is_val e' ∧ P e') ∨ ∃ e'', step e' e''.
+
+  Lemma Safe_mono (P Q : expr → Prop) e : (∀ v, P v → Q v) → Safe P e → Safe Q e.
+  Proof. unfold Safe; firstorder. Qed.
+
+  Lemma Safe_val (P : expr → Prop) e : is_val e → P e → Safe P e.
+  Proof.
+    unfold Safe; intros He HPe e' Hstp.
+    left.
+    apply val_steps_eq in Hstp; subst; auto.
+  Qed.
+
+  Lemma Safe_val_inv (P : expr → Prop) e : is_val e → Safe P e → P e.
+  Proof.
+    unfold Safe; intros He HSf.
+    destruct (HSf e) as [|[e' He']]; [apply steps_refl|tauto|].
+    contradict He'; apply val_no_step; trivial.
+  Qed.
+
+  Lemma Safe_step (P : expr → Prop) e e' : step e e' → Safe P e → Safe P e'.
+  Proof.
+    intros Hstep HSf ei Hsteps.
+    apply HSf.
+    apply steps_eq_or_step_iff; eauto.
+  Qed.
+
+  Lemma det_head_step_det_step e e' : det_head_step e e' → det_step e e'.
+  Proof.
+    intros [Hhs Hdt]; split; [apply head_step_step; assumption|].
+    intros e'' Hstp.
+    inversion Hstp as [? ? ? ? Hhs']; subst.
+    apply ectx_head_step in Hhs as [Hid|Hvl]; [| |assumption].
+    - rewrite Hid; rewrite Hid in Hdt. apply Hdt; assumption.
+    - contradict Hhs'; apply is_val_no_head_step; trivial.
+  Qed.
+
+  Lemma Safe_det_step_back (P : expr → Prop) e e' : det_step e e' → Safe P e' → Safe P e.
+  Proof.
+    intros Hdstep HSf ei Hsteps.
+    apply steps_eq_or_step_iff in Hsteps as [->|(e'' & He''1 & He''2)].
+    - right; eexists; apply Hdstep.
+    - apply Hdstep in He''1; subst.
+      apply HSf; assumption.
+  Qed.
+
+  Lemma Safe_head_step_back (P : expr → Prop) e e' : det_head_step e e' → Safe P e' → Safe P e.
+  Proof.
+    intros.
+    eapply Safe_det_step_back; [apply det_head_step_det_step|]; eassumption.
+  Qed.
+
+  Lemma Safe_bind (P Q : expr → Prop) e K :
+    is_ectx K → Safe P e → (∀ v, is_val v → P v → Safe Q (K v)) → Safe Q (K e).
+  Proof.
+    intros HK He HKSf e' Hstps.
+    remember (K e) as Ke.
+    revert e HeqKe He.
+    pattern Ke; pattern e'.
+    match goal with
+    | |- (λ e2, (λ e1, ?P) _) _ => simpl; apply (steps_ind (λ e1 e2, P))
+    end; [| |assumption]; clear e' Ke Hstps.
+    - intros ? e ? He; subst.
+      destruct (is_val_dec (K e)).
+      + assert (is_val e) by (eapply is_val_under_ectx; eauto).
+        eapply (HKSf e);
+          [assumption|eapply Safe_val_inv; assumption| apply steps_refl].
+      + destruct (is_val_dec e).
+        * eapply (HKSf e);
+          [assumption|eapply Safe_val_inv; assumption| apply steps_refl].
+        * destruct (He e) as [|[e' He']]; [apply steps_refl|tauto|].
+          right; eexists; apply ectx_step; eauto.
+    - intros e e' e'' Hstp Hstps IHstps ei ? Hei; subst.
+      pose proof Hstp as Hvlstp; apply step_under_ectx in Hvlstp as [Hvl|[e3 [He31 He32]]];
+        [|subst|assumption].
+      + eapply (HKSf ei);
+          [assumption|eapply Safe_val_inv; assumption| apply steps_eq_or_step_iff; eauto].
+      + eapply IHstps; [reflexivity|].
+        eapply Safe_step; eauto.
+  Qed.
+
+  Definition Normalizes (P : expr → Prop) (e : expr) := ∃ v, is_val v ∧ steps e v ∧ P v.
+
+  Lemma Normalizes_mono (P Q : expr → Prop) e : (∀ v, P v → Q v) → Normalizes P e → Normalizes Q e.
+  Proof. unfold Safe; firstorder. Qed.
+
+  Lemma Normalizes_val (P : expr → Prop) e : is_val e → P e → Normalizes P e.
+  Proof.
+    intros ? ?; eexists; repeat split; [eassumption|apply steps_refl|eassumption].
+  Qed.
+
+  Lemma Normalizses_val_inv (P : expr → Prop) e : is_val e → Normalizes P e → P e.
+  Proof.
+    intros Hiv (e' & He'1 & He'2 & He'3).
+    apply val_steps_eq in He'2; [subst; trivial|assumption].
+  Qed.
+
+  Lemma Normalizes_step_back (P : expr → Prop) e e' : step e e' → Normalizes P e' → Normalizes P e.
+  Proof.
+    intros Hstep (v & Hv1 & Hv2 & Hv3).
+    exists v; repeat split; [assumption| |assumption].
+    apply steps_eq_or_step_iff; eauto.
+  Qed.
+
+  Lemma Normalizes_head_step_back (P : expr → Prop) e e' :
+    head_step e e' → Normalizes P e' → Normalizes P e.
+  Proof.
+    intros Hstep (v & Hv1 & Hv2 & Hv3).
+    exists v; repeat split; [assumption| |assumption].
+    apply steps_eq_or_step_iff; eauto using head_step_step.
+  Qed.
+
+  Lemma Normalizes_det_step (P : expr → Prop) e e' :
+    det_step e e' → Normalizes P e → Normalizes P e'.
+  Proof.
+    intros Hdstep (v & Hv1 & Hv2 & Hv3).
+    exists v; repeat split; [assumption| |assumption].
+    apply steps_eq_or_step_iff in Hv2 as [->|(e'' & He''1 & He''2)].
+    - destruct Hdstep as [Hstp%val_no_step ?]; tauto.
+    - pose proof He''1 as ->%Hdstep; assumption.
+  Qed.
+
+  Lemma Normalizes_bind (P Q : expr → Prop) e K :
+    is_ectx K → Normalizes P e → (∀ v, is_val v → P v → Normalizes Q (K v)) → Normalizes Q (K e).
+  Proof.
+    intros HK He HKnrm.
+    destruct He as (v & Hv1 & Hv2 & Hv3).
+    destruct (HKnrm v) as (w & Hw1 & Hw2 & Hw3); [assumption|assumption|].
+    exists w; repeat split; [assumption| |assumption].
+    eapply steps_trans; [|eassumption].
+    apply ectx_steps; assumption.
+  Qed.
+
+End language.
