theories/stlc_cbv_normalization.v
@@ -1,0 +1,77 @@
+From Coq.Unicode Require Import Utf8.
+From Coq.Lists Require Import List.
+From Autosubst Require Import Autosubst.
+From Coq.Relations Require Import Relations.
+From ShortLogrels Require Import prelude language stlc_cbv.
+
+Fixpoint val_rel (τ : type) (v : expr) : Prop :=
+  match τ with
+  | TUnit => v = TT
+  | TProd τ1 τ2 => ∃ v1 v2, v = Pair v1 v2 ∧ val_rel τ1 v1 ∧ val_rel τ2 v2
+  | TFun τ1 τ2 => is_val v ∧ ∀ w, val_rel τ1 w → Normalizes (val_rel τ2) (App v w)
+  end.
+
+Lemma val_rel_is_val τ v : val_rel τ v → is_val v.
+Proof.
+  revert v; induction τ; intros v; simpl in *; subst.
+  - intros ?; subst; constructor.
+  - firstorder; subst; constructor; auto.
+  - intuition.
+Qed.
+
+Definition expr_rel (τ : type) (e : expr) := Normalizes (val_rel τ) e.
+
+Theorem Fundamental Γ e τ :
+  typed Γ e τ → ∀ env, env_rel val_rel Γ env → expr_rel τ e.[env_subst env].
+Proof.
+  intros Htp.
+  induction Htp; intros env Henv; simpl.
+  - simpl.
+    assert (val_rel tp (env_subst env v)).
+    { eapply env_rel_lookup1 in Henv as [? [? ?]]; [|eauto; fail].
+      erewrite env_subst_lookup; eauto. }
+    apply Normalizes_val; [eapply val_rel_is_val; eauto|assumption].
+  - apply Normalizes_val; [constructor|simpl; trivial].
+  - eapply (Normalizes_bind _ _ _ (λ e, Pair e _));
+      [repeat econstructor; fail|apply IHHtp1; trivial; fail|].
+    intros v1 Hv11 Hv12.
+    eapply (Normalizes_bind _ _ _ (λ e, Pair _ e)); [|apply IHHtp2; trivial; fail|].
+    { repeat econstructor; trivial. }
+    intros v2 Hv21 Hv22.
+    apply Normalizes_val; [constructor; trivial; fail|eexists _, _; eauto].
+  - eapply (Normalizes_bind _ _ _ (λ e, Fst e));
+      [repeat econstructor; fail|apply IHHtp; trivial; fail|].
+    intros v Hv1 (v1 & v2 & -> & Hv1r & Hv2r).
+    inversion Hv1; subst.
+    eapply Normalizes_head_step_back; [constructor; auto; fail|].
+    apply Normalizes_val; assumption.
+  - eapply (Normalizes_bind _ _ _ (λ e, Snd e));
+      [repeat econstructor; fail|apply IHHtp; trivial; fail|].
+    intros v Hv1 (v1 & v2 & -> & Hv1r & Hv2r).
+    inversion Hv1; subst.
+    eapply Normalizes_head_step_back; [constructor; auto; fail|].
+    apply Normalizes_val; assumption.
+  - apply Normalizes_val; [constructor; fail|].
+    split; [constructor; fail|].
+    intros w Hw.
+    assert (is_val w) by (eapply val_rel_is_val; eauto).
+    eapply Normalizes_head_step_back; [constructor; auto; fail|].
+    asimpl.
+    apply (IHHtp (_ :: _)).
+    apply env_rel_cons; assumption.
+  - eapply (Normalizes_bind _ _ _ (λ e, App e _));
+      [repeat econstructor; fail|apply IHHtp1; trivial; fail|].
+    intros v1 Hv11 Hv12.
+    eapply (Normalizes_bind _ _ _ (λ e, App _ e)); [|apply IHHtp2; trivial; fail|].
+    { repeat econstructor; trivial. }
+    intros v2 Hv21 Hv22.
+    apply Hv12; trivial.
+Qed.
+
+Corollary type_safety e τ : typed nil e τ → Normalizes (λ _, True) e.
+Proof.
+  intros Htp.
+  eapply Normalizes_mono; [tauto|].
+  replace e with e.[env_subst nil] by (asimpl; reflexivity).
+  eapply (Fundamental nil); [eassumption|apply env_rel_nil].
+Qed.
